src/Framework/Label.v
@@ -13,7 +13,6 @@ Module A1 := ANF1.
 (* Attach Unique Labels *)
 
 (* Specification *)
-(*
 Inductive trans (Γ : A0.vars) : label -> A0.exp -> label -> A1.exp -> Prop :=
 | Trans_ret :
   forall {x l0},
@@ -21,7 +20,7 @@ Inductive trans (Γ : A0.vars) : label -> A0.exp -> label -> A1.exp -> Prop :=
     trans Γ l0 (A0.Eret x) l0 (A1.Eret x)
 
 | Trans_fun :
-  forall {f xs e0 k0 e1 k1 l0 l2 l3},
+  forall l2 {f xs e0 k0 e1 k1 l0 l3},
     let l1 := next_label l0 in
     trans (FromList xs :|: (f |: Γ)) l1 e0 l2 e1 ->
     trans (f |: Γ) l2 k0 l3 k1 ->
@@ -56,34 +55,389 @@ Inductive trans (Γ : A0.vars) : label -> A0.exp -> label -> A1.exp -> Prop :=
     trans (x |: Γ) l1 k0 l2 k1 ->
     trans Γ l0 (A0.Eproj x n y k0) l2 (A1.Eproj x l0 n y k1)
 
-| Trans_case_nil :
-  forall {x l0},
+| Trans_case :
+  forall l2 {x cl0 cl1 l0},
     (x \in Γ) ->
     let l1 := next_label l0 in
-    trans Γ l0 (A0.Ecase x []) l1 (A1.Ecase x l0 [])
+    trans_case Γ l1 cl0 l2 cl1 ->
+    trans Γ l0 (A0.Ecase x cl0) l2 (A1.Ecase x l0 cl1)
+
+with trans_case (Γ : A0.vars) : label -> list (A0.ctor_tag * A0.exp) -> label -> list (A1.ctor_tag * A1.exp) -> Prop :=
+| Trans_case_nil :
+  forall {l0},
+    trans_case Γ l0 [] l0 []
 
 | Trans_case_cons :
-  forall {x e0 e1 t cl0 cl1 l0 l2 l4},
-    (x \in Γ) ->
-    let l1 := next_label l0 in
-    trans Γ l1 e0 l2 e1 ->
-    let l3 := next_label l2 in
-    trans Γ l3 (A0.Ecase x cl0) l4 (A1.Ecase x l2 cl1) ->
-    trans Γ l0 (A0.Ecase x ((t, e0) :: cl0)) l4 (A1.Ecase x l0 ((t, e1) :: cl1)).
+  forall l1 l2 {l0 e0 e1 t cl0 cl1},
+    trans Γ l0 e0 l1 e1 ->
+    trans_case Γ l1 cl0 l2 cl1 ->
+    trans_case Γ l0 ((t, e0) :: cl0) l2 ((t, e1) :: cl1).
 
 Hint Constructors trans : core.
+Hint Constructors trans_case : core.
+
+Scheme trans_mut := Induction for trans Sort Prop
+with trans_case_mut := Induction for trans_case Sort Prop.
+
+Lemma trans_label_le Γ l1 e1 l2 e2 :
+  trans Γ l1 e1 l2 e2 ->
+  Pos.le l1 l2.
+Proof.
+  intro H.
+  induction H using trans_mut with (P0 := fun Γ l0 cl0 l1 cl1 tr =>
+                                            Pos.le l0 l1);
+    simpl; intros;
+    try Pos.order;
+    try (pose proof (next_label_le l0); subst l1; eauto;
+         Pos.order).
+Qed.
+
+Lemma trans_case_label_le Γ l1 cl1 l2 cl2 :
+  trans_case Γ l1 cl1 l2 cl2 ->
+  Pos.le l1 l2.
+Proof.
+  intro H.
+  induction H; simpl; intros; eauto;
+    try Pos.order.
+  eapply trans_label_le in H; eauto.
+  Pos.order.
+Qed.
+
+Lemma has_label_case cl:
+  forall l0 l x,
+    has_label (Ecase x l0 cl) l ->
+    (l0 = l \/
+     Exists (fun '(_, e) => l \in (has_label e)) cl).
+Proof.
+  induction cl; simpl; intros.
+  - inv H.
+    left; auto.
+  - inv H.
+    + left; auto.
+    + right; auto.
+    + eapply IHcl in H5; eauto.
+      inv H5.
+      * left; eauto.
+      * right.
+        apply Exists_cons.
+        right; auto.
+Qed.
+
+Lemma trans_label_inv Γ l1 e1 l2 e2 :
+  trans Γ l1 e1 l2 e2 ->
+  forall l,
+    (l \in has_label e2) ->
+    (Pos.le l1 l /\ Pos.lt l l2).
+Proof.
+  intro H.
+  induction H using trans_mut with (P0 := fun Γ l0 cl0 l1 cl1 tr =>
+                                            forall l,
+                                              Exists (fun '(t, e) => (l \in has_label e)) cl1 ->
+                                              (Pos.le l0 l /\ Pos.lt l l1));
+  simpl; intros.
+  - inv H.
+  - inv H1;
+      apply trans_label_le in H;
+      apply trans_label_le in H0.
+    + split; try (eapply Pos.le_refl; eauto).
+      pose proof (next_label_lt l); subst l1.
+      Pos.order.
+    + pose proof (next_label_lt l0); subst l1.
+      split;
+        eapply IHtrans1 in H8; eauto; inv H8;
+        Pos.order.
+    + pose proof (next_label_lt l0); subst l1.
+      split;
+        eapply IHtrans2 in H8; eauto; inv H8;
+        Pos.order.
+  - inv H.
+    split; try Pos.order.
+    eapply next_label_lt; eauto.
+  - eapply trans_label_le in H; eauto.
+    inv H0.
+    + split; try Pos.order.
+      pose proof (next_label_lt l); subst l1.
+      Pos.order.
+    + eapply IHtrans in H7; eauto; inv H7.
+      pose proof (next_label_lt l0); subst l1.
+      split; Pos.order.
+  - eapply trans_label_le in H; eauto.
+    inv H0.
+    + split; try Pos.order.
+      pose proof (next_label_lt l); subst l1.
+      Pos.order.
+    + eapply IHtrans in H7; eauto; inv H7.
+      pose proof (next_label_lt l0); subst l1.
+      split; Pos.order.
+  - eapply trans_label_le in H; eauto.
+    inv H0.
+    + split; try Pos.order.
+      pose proof (next_label_lt l); subst l1.
+      Pos.order.
+    + eapply IHtrans in H7; eauto; inv H7.
+      pose proof (next_label_lt l0); subst l1.
+      split; Pos.order.
+  - inv H.
+    + split; try Pos.order.
+      eapply trans_case_label_le in t; eauto.
+      pose proof (next_label_lt l); subst l1.
+      Pos.order.
+    + assert (Hl : (l1 <= l < l2)%positive) by (eapply IHtrans; eauto).
+      inv Hl.
+      pose proof (next_label_lt l0); subst l1.
+      split; Pos.order.
+    + eapply has_label_case in H4; eauto.
+      inv H4.
+      * split; try (eapply Pos.le_refl; eauto).
+        eapply trans_case_label_le in t; eauto.
+        eapply Pos.lt_le_trans; eauto.
+        eapply next_label_lt; eauto.
+      * assert (Hl : (l1 <= l < l2)%positive) by (eapply IHtrans; eauto).
+        inv Hl.
+        split; auto.
+        eapply Pos.le_trans; eauto.
+        eapply next_label_le; eauto.
+  - apply Exists_nil in H; inv H.
+  - inv H0.
+    + apply IHtrans in H2; inv H2.
+      split; auto.
+      eapply Pos.lt_le_trans; eauto.
+      eapply trans_case_label_le; eauto.
+    + apply IHtrans0 in H2; inv H2.
+      split; auto.
+      eapply Pos.le_trans; eauto.
+      eapply trans_label_le; eauto.
+Qed.
+
+Lemma trans_case_label_inv Γ l1 cl1 l2 cl2 :
+  trans_case Γ l1 cl1 l2 cl2 ->
+  forall l,
+    Exists (fun '(_, e) => (l \in has_label e)) cl2 ->
+    (Pos.le l1 l /\ Pos.lt l l2).
+Proof.
+  intros H.
+  induction H; simpl; intros; eauto.
+  - inv H.
+  - inv H1.
+    + eapply trans_label_inv in H; eauto; inv H.
+      eapply trans_case_label_le in H0; eauto.
+      split; Pos.order.
+    + eapply IHtrans_case in H3; eauto; inv H3.
+      split; auto.
+      eapply trans_label_le in H; eauto.
+      Pos.order.
+Qed.
+
+(*
+Lemma trans_label_inv_r Γ l1 e1 l2 e2 :
+  trans Γ l1 e1 l2 e2 ->
+  forall l,
+    (Pos.le l1 l /\ Pos.lt l l2) ->
+    (l \in has_label e2).
+Proof.
+    intro H.
+    induction H using trans_mut with (P0 := fun Γ l0 cl0 l1 cl1 tr =>
+                                              forall l,
+                                                (Pos.le l0 l /\ Pos.lt l l1) ->
+                                                Exists (fun '(t, e) => (l \in has_label e)) cl1);
+      simpl; intros.
+    -
+Admitted.
+*)
+(*
+Lemma not_has_label_case cl l0 l x:
+  l0 <> l ->
+  Forall (fun '(_, e) => ~ (l \in (has_label e))) cl ->
+  ~ (has_label (Ecase x l0 cl) l).
+Proof.
+  intros.
+  generalize dependent l0.
+  revert x.
+  induction H0; simpl; intros; intros Hc; inv Hc; eauto.
+  eapply IHForall; eauto.
+Qed.
+
+Lemma trans_label_inv Γ l1 e1 l2 e2 :
+  trans Γ l1 e1 l2 e2 ->
+  forall l,
+    Pos.lt l l1 ->
+    ~ (l \in has_label e2).
+Proof.
+  intro H.
+  induction H using trans_mut with (P0 := fun Γ l0 cl0 l1 cl1 tr =>
+                                            forall l,
+                                              Pos.lt l l0 ->
+                                              Forall (fun '(t, e) => ~ (l \in has_label e)) cl1);
+  simpl; intros; eauto.
+  - intros Hc.
+    inv Hc.
+  - intros Hc.
+    inv Hc.
+    + eapply Pos.lt_irrefl; eauto.
+    + eapply (IHtrans1 l); eauto.
+      eapply Pos.lt_trans; eauto.
+      eapply next_label_lt; eauto.
+    + eapply (IHtrans2 l); eauto.
+      eapply Pos.lt_trans; eauto.
+      apply trans_label_le in H.
+      eapply Pos.lt_le_trans; eauto.
+      eapply next_label_lt; eauto.
+  - intro Hc.
+    inv Hc.
+    eapply Pos.lt_irrefl; eauto.
+  - intros Hc.
+    inv Hc.
+    + eapply Pos.lt_irrefl; eauto.
+    + eapply IHtrans; eauto.
+      eapply Pos.lt_trans; eauto.
+      eapply next_label_lt; eauto.
+  - intros Hc.
+    inv Hc.
+    + eapply Pos.lt_irrefl; eauto.
+    + eapply IHtrans; eauto.
+      eapply Pos.lt_trans; eauto.
+      eapply next_label_lt; eauto.
+  - intros Hc.
+    inv Hc.
+    + eapply Pos.lt_irrefl; eauto.
+    + eapply IHtrans; eauto.
+      eapply Pos.lt_trans; eauto.
+      eapply next_label_lt; eauto.
+  - intros Hc.
+    inv Hc.
+    + eapply Pos.lt_irrefl; eauto.
+    + assert (Hl: Pos.lt l l1).
+      {
+        eapply Pos.lt_trans; eauto.
+        eapply next_label_lt; eauto.
+      }
+      eapply IHtrans in Hl; eauto.
+      inv Hl.
+      eapply H2; eauto.
+    + assert (Hl: Pos.lt l l1).
+      {
+        eapply Pos.lt_trans; eauto.
+        eapply next_label_lt; eauto.
+      }
+      eapply IHtrans in Hl; eauto.
+      inv Hl.
+      eapply not_has_label_case; eauto.
+      intros Hc; subst.
+      eapply Pos.lt_irrefl; eauto.
+  - constructor; auto.
+    eapply IHtrans0; eauto.
+    eapply Pos.lt_le_trans; eauto.
+    eapply trans_label_le; eauto.
+Qed.
+ *)
 
 Lemma trans_unique_label Γ l1 e1 l2 e2 :
   trans Γ l1 e1 l2 e2 ->
   unique_label e2.
 Proof.
   intro H.
-  induction H; simpl; intros; eauto.
-  - econstructor; eauto.
-Abort.
- *)
 
-(* Note this is directly based on `unique_label` *)
+  induction H using trans_mut with (P0 := fun Γ l0 cl0 l1 cl1 tr =>
+                                            Forall (fun '(t, e) => unique_label e) cl1);
+  simpl; intros; eauto.
+  - econstructor; eauto.
+    + intro Hc.
+      eapply trans_label_inv in H; eauto; inv H.
+      pose proof (next_label_lt l0); subst l1.
+      Pos.order.
+    + intros Hc.
+      eapply trans_label_inv in H0; eauto; inv H0.
+      pose proof (next_label_lt l0); subst l1.
+      eapply trans_label_le in H.
+      Pos.order.
+    + constructor; intros.
+      intros Hc.
+      inv Hc.
+      eapply trans_label_inv in H; eauto; inv H.
+      eapply trans_label_inv in H0; eauto; inv H0.
+      Pos.order.
+  - econstructor; eauto.
+    intros Hc.
+    eapply trans_label_inv in H; eauto; inv H.
+    pose proof (next_label_lt l0); subst l1.
+    Pos.order.
+  - econstructor; eauto.
+    intros Hc.
+    eapply trans_label_inv in H; eauto; inv H.
+    pose proof (next_label_lt l0); subst l1.
+    Pos.order.
+  - econstructor; eauto.
+    intros Hc.
+    eapply trans_label_inv in H; eauto; inv H.
+    pose proof (next_label_lt l0); subst l1.
+    Pos.order.
+  - generalize dependent l0.
+    induction t; simpl; eauto.
+    inv IHtrans.
+    econstructor; eauto.
+    + intros Hc.
+      eapply trans_label_inv in H0; eauto; inv H0.
+      Pos.order.
+    + admit.
+    +
+
+
+    generalize dependent cl0.
+    revert l0 l1 l2 x i.
+    induction IHtrans; intros; eauto.
+    destruct x.
+    econstructor; eauto.
+    + intros Hc.
+      eapply trans_case_label_inv in t; eauto; inv t.
+      pose proof (next_label_lt l0); subst l1.
+      Pos.order.
+    + admit.
+    + inv t.
+      eapply IHIHtrans; eauto.
+      inv t.
+Abort.
+
+        assert (Hl : ~ (l0 <= l < l1)%positive).
+        {
+          intros Hc.
+          apply H1.
+          eapply trans_label_inv_r; eauto.
+        }
+        split; auto.
+
+
+        assert (Hl' : ~ (l0 <= l)%positive).
+        {
+          intros Hc.
+          apply Hl.
+          split; auto.
+
+        }
+
+        split; auto.
+
+
+      }
+      inv Hl.
+      split; auto.
+      eapply Pos.le_trans; eauto.
+      eapply next_label_le; eauto.
+    +
+Abort.
+
+      eapply trans_label_le in t; eauto.
+      eapply Pos.lt_le_trans; eauto.
+      eapply next_label_lt; eauto.
+    + eapply IHtrans in H7; eauto.
+      inv H7.
+      split; auto.
+      eapply Pos.le_trans; eauto.
+      eapply next_label_le; eauto.
+  -
+
+(*
+(* Note this is directly based on `unique_label`
+   However, this isn't sufficient to show linking compat *)
 Inductive trans (Γ : A0.vars) : A0.exp -> A1.exp -> Prop :=
 | Trans_ret :
   forall {x},
@@ -146,3 +500,4 @@ Proof.
   intro H.
   induction H; intros; eauto.
 Qed.
+*)
